1.  Rationalize mapsto, field_mapsto, etc, as follows:    umapsto:   untyped mapsto, meaning that the contents            might be undefined or wrong type    mapsto:   maps to a value of the right type    mapsto_:  maps to any thing, like  p |-> _  in standard notation    field_mapsto:  the named field maps to a well-typed value    field_mapsto_:  the named field contains anything at all
2. Write sumarray.c, that exercises arrays
    and verif_sumarray.v, that proves adding-up-an-array

progs/sumarray.c
@@ -1,0 +1,22 @@
+#include <stddef.h>
+
+int sumarray(int a[], int n) {
+  int i,s,x;
+  i=0;
+  s=0;
+  while (i<n) {
+    x=a[i];
+    s+=x;
+    i++;
+  }
+  return s;
+}
+
+int four[4] = {1,2,3,4};
+
+int main(void) {
+  int s;
+  s = sumarray(four,4);
+  return s;
+}
+
