progs/sumarray.v
@@ -1,0 +1,90 @@
+Require Import Clightdefs.
+
+Local Open Scope Z_scope.
+
+Definition _s : ident := 7%positive.
+Definition ___builtin_annot_intval : ident := 3%positive.
+Definition ___builtin_fabs : ident := 1%positive.
+Definition _sumarray : ident := 9%positive.
+Definition _a : ident := 4%positive.
+Definition _x : ident := 8%positive.
+Definition _i : ident := 6%positive.
+Definition _main : ident := 11%positive.
+Definition _n : ident := 5%positive.
+Definition ___builtin_memcpy_aligned : ident := 2%positive.
+Definition _four : ident := 10%positive.
+
+
+Definition f_sumarray := {|
+  fn_return := tint;
+  fn_params := ((_a, (tptr tint)) :: (_n, tint) :: nil);
+  fn_vars := nil;
+  fn_temps := ((_i, tint) :: (_s, tint) :: (_x, tint) :: nil);
+  fn_body :=
+(Ssequence
+  (Sset _i (Econst_int (Int.repr 0) tint))
+  (Ssequence
+    (Sset _s (Econst_int (Int.repr 0) tint))
+    (Ssequence
+      (Swhile
+        (Ebinop Olt (Etempvar _i tint) (Etempvar _n tint) tint)
+        (Ssequence
+          (Sset _x
+            (Ederef
+              (Ebinop Oadd (Etempvar _a (tptr tint)) (Etempvar _i tint)
+                (tptr tint)) tint))
+          (Ssequence
+            (Sset _s
+              (Ebinop Oadd (Etempvar _s tint) (Etempvar _x tint) tint))
+            (Sset _i
+              (Ebinop Oadd (Etempvar _i tint) (Econst_int (Int.repr 1) tint)
+                tint)))))
+      (Sreturn (Some (Etempvar _s tint))))))
+|}.
+
+Definition v_four := {|
+  gvar_info := (tarray tint 4);
+  gvar_init := (Init_int32 (Int.repr 1) :: Init_int32 (Int.repr 2) ::
+                Init_int32 (Int.repr 3) :: Init_int32 (Int.repr 4) :: nil);
+  gvar_readonly := false;
+  gvar_volatile := false
+|}.
+
+Definition f_main := {|
+  fn_return := tint;
+  fn_params := nil;
+  fn_vars := nil;
+  fn_temps := ((_s, tint) :: (12%positive, tint) :: nil);
+  fn_body :=
+(Ssequence
+  (Ssequence
+    (Scall (Some 12%positive)
+      (Evar _sumarray (Tfunction (Tcons (tptr tint) (Tcons tint Tnil)) tint))
+      ((Evar _four (tarray tint 4)) :: (Econst_int (Int.repr 4) tint) :: nil))
+    (Sset _s (Etempvar 12%positive tint)))
+  (Sreturn (Some (Etempvar _s tint))))
+|}.
+
+Definition prog : Clight.program := {|
+prog_defs :=
+((___builtin_fabs,
+   Gfun(External (EF_builtin ___builtin_fabs
+                   (mksignature (AST.Tfloat :: nil) (Some AST.Tfloat)))
+     (Tcons tdouble Tnil) tdouble)) ::
+ (___builtin_memcpy_aligned,
+   Gfun(External (EF_builtin ___builtin_memcpy_aligned
+                   (mksignature
+                     (AST.Tint :: AST.Tint :: AST.Tint :: AST.Tint :: nil)
+                     None))
+     (Tcons (tptr tvoid)
+       (Tcons (tptr tvoid) (Tcons tuint (Tcons tuint Tnil)))) tvoid)) ::
+ (___builtin_annot_intval,
+   Gfun(External (EF_builtin ___builtin_annot_intval
+                   (mksignature (AST.Tint :: AST.Tint :: nil)
+                     (Some AST.Tint)))
+     (Tcons (tptr tschar) (Tcons tint Tnil)) tint)) ::
+ (_sumarray, Gfun(Internal f_sumarray)) :: (_four, Gvar v_four) ::
+ (_main, Gfun(Internal f_main)) :: nil);
+prog_main := _main
+|}.
+
