progs/verif_sumarray.v
@@ -1,0 +1,296 @@
+Load loadpath.
+Require Import Coqlib msl.Coqlib2.
+Require Import veric.SeparationLogic.
+Require Import Ctypes.
+Require Import Clightdefs.
+Require veric.SequentialClight.
+Import SequentialClight.SeqC.CSL.
+Require Import progs.field_mapsto.
+Require Import progs.client_lemmas.
+Require Import progs.assert_lemmas.
+Require Import progs.forward.
+Require Import progs.malloc_lemmas.
+Require Import progs.sumarray.
+
+Local Open Scope logic.
+
+
+Fixpoint rangespec' (lo: Z) (n: nat) (P: Z -> mpred): mpred :=
+  match n with
+  | O => emp
+  | S n' => P lo * rangespec' (Zsucc lo) n' P
+ end.
+
+Definition rangespec (lo hi: Z) (P: Z -> mpred) : mpred :=
+  rangespec' lo (nat_of_Z (hi-lo)) P.
+
+Definition repable (z: Z) := Int.signed (Int.repr z)=z.
+Definition repable_dec (z: Z) : {repable z}+{~repable z}.
+Proof.
+ intros. apply zeq.
+Defined.
+
+Definition add_ptr_int' (ty: type) (v: val) (i: Z) : val :=
+  if repable_dec (sizeof ty * i)
+   then match v with
+      | Vptr b ofs => 
+           Vptr b (Int.add ofs (Int.repr (sizeof ty * i)))
+      | _ => Vundef
+      end
+  else Vundef.
+
+Definition add_ptr_int (ty: type) (v: val) (i: Z) : val :=
+           eval_binop Oadd (tptr ty) tint v (Vint (Int.repr i)).
+Lemma repable_mult2:
+  forall i j, i<>0 -> repable (i*j) -> repable j.
+Admitted.
+Lemma repable_mult1:
+  forall i j, j<>0 -> repable (i*j) -> repable i.
+Proof.
+intros.
+ rewrite Zmult_comm in H0.
+ apply repable_mult2 in H0; auto.
+Qed.
+
+Lemma add_ptr_tint_eq:
+  forall ty v i, repable (sizeof ty * i) ->
+       add_ptr_int' ty v i = add_ptr_int ty v i.
+Proof.
+ intros.
+ unfold add_ptr_int, add_ptr_int'.
+ rewrite if_true by auto.
+ destruct v; simpl; auto.
+ unfold eval_binop; simpl; auto.
+ f_equal. f_equal.
+ destruct (eq_dec i 0).
+    subst. rewrite Int.mul_zero. rewrite Zmult_0_r. auto.
+ assert (repable (sizeof ty)). eapply repable_mult1; eauto.
+ assert (repable i). apply repable_mult2 in H; auto.
+        pose proof (sizeof_pos ty); omega.
+ unfold repable in *.
+ rewrite Int.mul_signed. 
+ rewrite <- H.
+ repeat rewrite Int.repr_signed.
+ rewrite H0. rewrite H1. auto.
+Qed.
+
+Definition array_at (t: type) (sh: Share.t) (v: val) (i: Z) (e: reptype t) : mpred :=
+   typed_mapsto t sh 0 (add_ptr_int t v i) e.
+
+Definition array_at_range (t: type) (sh: Share.t) (f: Z -> reptype t) (lo hi: Z)
+                                   (v: val) :=
+           rangespec lo hi (fun i => array_at t sh v i (f i)).
+
+Fixpoint fold_range' {A: Type} (f: Z -> A -> A) (zero: A) (lo: Z) (n: nat) : A :=
+ match n with
+  | O => zero
+  | S n' => f lo (fold_range' f  zero (Zsucc lo) n')
+ end.
+
+Definition fold_range {A: Type} (f: Z -> A -> A) (zero: A) (lo hi: Z) : A :=
+  fold_range' f zero lo (nat_of_Z (hi-lo)).
+
+Definition add_elem (f: Z -> int) (i: Z) := Int.add (f i).
+
+Definition sumarray_spec :=
+ DECLARE _sumarray
+  WITH a0: val, sh : share, contents : Z -> int, size: Z
+  PRE [ _a OF (tptr tint), _n OF tint ] 
+          !! (0 <= size <= Int.max_signed) &&
+          local (`(eq a0) (eval_id _a)) &&
+          local (`(eq (Vint (Int.repr size))) (eval_id _n))   &&
+          local (`denote_tc_isptr (eval_id _a)) &&
+          `(array_at_range tint sh contents 0 size) (eval_id _a)
+  POST [ tint ]  
+    local (`(eq (Vint (fold_range (add_elem contents) Int.zero 0 size))) retval) &&
+            `(array_at_range tint sh contents 0 size a0).
+
+Definition main_spec :=
+ DECLARE _main
+  WITH u : unit
+  PRE  [] main_pre prog u
+  POST [ tint ] main_post prog u.
+
+Definition Vprog : varspecs := (_four, Tarray tint 4 noattr)::nil.
+
+Definition Gprog : funspecs := 
+    sumarray_spec :: main_spec::nil.
+
+Definition Gtot := do_builtins (prog_defs prog) ++ Gprog.
+
+Definition sumarray_Inv a0 sh contents size := 
+ EX i: Z,
+  (PROP  (0 <= i <= size)
+   LOCAL  (`(eq a0) (eval_id _a);   `(eq (Vint (Int.repr i))) (eval_id _i);
+                `(eq (Vint (Int.repr size))) (eval_id _n);
+           `denote_tc_isptr (eval_id _a); 
+    `(eq (Vint (fold_range (add_elem contents) Int.zero 0 i))) (eval_id _s))
+   SEP (`(array_at_range tint sh contents 0 size) (eval_id _a))).
+
+Lemma split3_array_at_range:
+  forall i ty sh contents lo hi v,
+       lo <= i < hi ->
+     array_at_range ty sh contents lo hi v =
+     array_at_range ty sh contents lo i v *
+     typed_mapsto ty sh 0 (add_ptr_int ty v i) (contents i) *
+     array_at_range ty sh contents (Zsucc i) hi v.
+Proof.
+ intros.
+Admitted.
+
+Lemma lift_split3_array_at_range:
+  forall i ty sh contents lo hi,
+       lo <= i < hi ->
+     array_at_range ty sh contents lo hi =
+     array_at_range ty sh contents lo i *
+     (fun v => typed_mapsto ty sh 0 (add_ptr_int ty v i) (contents i)) *
+     array_at_range ty sh contents (Zsucc i) hi.
+Proof.
+ intros. extensionality v. simpl. apply split3_array_at_range. auto.
+Qed.
+
+Lemma body_sumarray: semax_body Vprog Gtot f_sumarray sumarray_spec.
+Proof.
+start_function. destruct p as [[a0 sh] contents].
+name a _a.
+name n _n.
+name i _i.
+name s _s.
+name x _x.
+repeat rewrite andp_assoc.
+normalizex.
+forward.  (* i = 0; *) 
+forward.  (* s = 0; *)
+forward_while (sumarray_Inv a0 sh contents size)
+    (PROP() LOCAL (`(eq a0) (eval_id _a);   
+     `(eq (Vint (fold_range (add_elem contents) Int.zero 0 size))) (eval_id _s))
+     SEP (`(array_at_range tint sh contents 0 size) (eval_id _a))).
+(* Prove that current precondition implies loop invariant *)
+unfold sumarray_Inv.
+apply exp_right with 0.
+go_lower. subst. normalize.
+ repeat apply andp_right; auto; apply prop_right; auto; omega.
+(* Prove that loop invariant implies typechecking condition *)
+go_lower.
+(* Prove that invariant && not loop-cond implies postcondition *)
+go_lower.  subst.
+ repeat apply andp_right; try apply prop_right; repeat split; auto.
+ f_equal. simpl in H2.
+ assert (~ (i0 < size)); [ | omega]. 
+ admit.  (* arithmetic proof *)
+(* Prove that loop body preserves invariant *)
+apply semax_pre_PQR with
+ (PROP (0 <= i0 < size) 
+  LOCAL (`(eq a0) (eval_id _a); `(eq (Vint (Int.repr i0))) (eval_id _i);
+   `(eq (Vint (Int.repr size))) (eval_id _n); `denote_tc_isptr (eval_id _a);
+   `(eq (Vint (fold_range (add_elem contents) Int.zero 0 i0))) (eval_id _s))
+   SEP  (`(array_at_range tint sh contents 0 size) (eval_id _a))).
+go_lower. subst. simpl in H2. apply andp_right; auto.
+apply prop_right; repeat split; auto; try omega.
+ admit.  (* arithmetic proof *)
+apply semax_extract_PROP; intro.
+apply semax_pre_PQR with
+(PROP  ()
+   LOCAL  (`(eq a0) (eval_id _a); `(eq (Vint (Int.repr i0))) (eval_id _i);
+   `(eq (Vint (Int.repr size))) (eval_id _n); `denote_tc_isptr (eval_id _a);
+   `(eq (Vint (fold_range (add_elem contents) Int.zero 0 i0))) (eval_id _s))
+   SEP 
+   (`(array_at_range tint sh contents 0 i0) (eval_id _a);
+    `(typed_mapsto tint sh 0) (`(eval_binop Oadd (tptr tint) tint)  (eval_id _a) (eval_id _i)) `(contents i0);
+    `(array_at_range tint sh contents (Zsucc i0) size) (eval_id _a))).
+rewrite typed_mapsto_tint.
+go_lower. subst.
+apply andp_right. apply prop_right; repeat split; auto.
+rewrite (split3_array_at_range i0) by omega.
+cancel.
+simpl_typed_mapsto.
+rewrite mapsto_offset_zero.
+auto.
+rewrite typed_mapsto_tint.
+forward. (* x = a[i]; *)
+forward. (* s += x; *)
+forward. (* i++; *)
+(* Prove postcondition of loop body implies loop invariant *)
+unfold sumarray_Inv.
+apply exp_right with (Zsucc i0).
+go_lower. subst. simpl in H3.
+ unfold eval_binop in H3; simpl in H3. inv H3.
+ unfold eval_binop in H2; simpl in H2.  inv H2.
+ apply andp_right. apply prop_right; repeat split; auto; try omega.
+ admit.  (* arithmetic proof *)
+ admit.  (* need simple lemma fold_range_split *)
+ rewrite split3_array_at_range with (i:=i0) (lo:=0)(hi:=size); auto.
+ simpl_typed_mapsto.
+ rewrite mapsto_offset_zero.
+ cancel.
+(* After the loop *)
+forward.  (* return s; *)
+go_lower.  subst; normalize.
+Qed.
+
+Definition four_contents (z: Z) : int := Int.repr (Zsucc z).
+
+Lemma  setup_globals:
+  forall u rho,  tc_environ (func_tycontext f_main Vprog Gtot) rho ->
+     main_pre prog u rho
+      |-- array_at_range tint Ews four_contents 0 4
+                (eval_var _four (tarray tint 4) rho).
+Proof.
+ unfold main_pre.
+ intros _ rho; normalize.
+ simpl.
+ destruct (globvar_eval_var _ _ _four _ H (eq_refl _) (eq_refl _))
+  as [b [z [H97 H99]]]. simpl in *.
+ unfold tarray.
+ rewrite H97.
+ unfold globvar2pred. simpl. rewrite H99. simpl.
+ unfold array_at_range, rangespec; simpl.
+ unfold array_at.
+ repeat  simpl_typed_mapsto.
+ rewrite sepcon_emp.
+ unfold four_contents. simpl.
+ change (umapsto  (Share.splice extern_retainer Share.top) (Tint I32 Unsigned noattr))
+       with (umapsto Ews tint).
+ replace (Vptr b z) with (Vptr b (Int.add z (Int.repr 0)))
+    by (rewrite Int.add_zero; auto).
+ repeat apply sepcon_derives; auto;
+ (repeat  rewrite Int.add_assoc; unfold mapsto;
+ apply andp_right; [apply prop_right; reflexivity | ];
+ match goal with
+  |- (umapsto _ _ (Vptr _ (Int.add z ?a)) _) |-- 
+      (umapsto _ _ (Vptr _ (Int.add z ?b)) _) =>
+     replace b with a; [auto | ]
+ end; compute; auto).
+Qed.
+
+
+Lemma body_main:  semax_body Vprog Gtot f_main main_spec.
+Proof.
+start_function.
+name s _s.
+apply (remember_value (eval_var _four (tarray tint 4))); intro a0.
+forward.  (*  r = sumarray(four,4); *)
+instantiate (1:= (a0,Ews,four_contents,4)) in (Value of witness).
+instantiate (1:=nil) in (Value of Frame).
+unfold Frame.
+ go_lower. normalize. eval_cast_simpl.
+ repeat apply andp_right; try apply prop_right; simpl; auto. 
+ compute; congruence.
+ simpl.
+ apply eval_var_isptr with Delta; simpl; auto.
+ apply setup_globals; auto.
+ forward.
+ forward. (* return s; *)
+ go_lower. subst. normalize.
+Qed.
+
+Lemma all_funcs_correct:
+  semax_func Vprog Gtot (prog_funct prog) Gtot.
+Proof.
+unfold Gtot, Gprog, prog, prog_funct; simpl.
+repeat (apply semax_func_cons_ext; [ reflexivity | apply semax_external_FF | ]).
+apply semax_func_cons; [ reflexivity | apply body_sumarray | ].
+apply semax_func_cons; [ reflexivity | apply body_main | ].
+apply semax_func_nil.
+Qed.
+
